coqart ch8 60%

coqart/ch8.v
@@ -1,12 +1,77 @@
 
 
-
-
-(** **** Exercise 8.5 *)
+(** ** Chapter 8. Inductive Predicates *)
 
 Require Import List.
 Import ListNotations.
 
+Require Import Relations.
+Require Import Le.
+Require Import ch5.
+
+(** **** Exercise 8.1 *)
+
+Inductive last (A : Set) : A -> list A -> Prop :=
+| last1 : forall a:A, last A a (a::nil)
+| last2 : forall (a x : A) (l : list A), last A a l -> last A a (x::l).
+
+Fixpoint last_fun (A : Set) (l : list A) : option A :=
+  match l with
+    | [] => None
+    | [a] => Some a
+    | h::t => last_fun A t
+  end.
+
+Theorem lasteq : forall (A : Set) (a : A) (l : list A),
+  last A a l <-> last_fun A l = Some a.
+Proof.
+  intros A a l.
+  generalize dependent a.
+  induction l as [|h t].
+  - split; intros H; inversion H.
+  - split; intros H. 
+    + simpl. destruct t as [|h' t'].
+      * inversion H. reflexivity.
+        inversion H2.
+      * apply IHt. inversion H. assumption.
+    + simpl in H. destruct t as [|h' t'].
+      * injection H. intros E. rewrite E. apply last1.
+      * apply last2. rewrite IHt. assumption.
+Qed.
+
+(** [] *)
+
+
+(** **** Exercise 8.2 *)
+
+Inductive palindrome (A : Set) : list A -> Prop :=
+| pal0 : palindrome A []
+| pal1 : forall x : A, palindrome A [x]
+| pal2 : forall (x : A) (l : list A), palindrome A l -> palindrome A ([x]++l++[x]).
+
+(** [] *)
+
+
+(** **** Exercise 8.3 *)
+(** [] *)
+
+
+(** **** Exercise 8.4 *)
+
+Inductive tsp (A : Set) : relation (list A) :=
+| tsp1 : forall (a b : A) (l : list A), tsp A (a::b::l) (b::a::l)
+| tsp2 : forall (x : A) (l1 l2 : list A), tsp A l1 l2 -> tsp A (x::l1) (x::l2).
+
+Inductive pmt (A : Set) : relation (list A) :=
+| pmt1 : forall (l1 l2 : list A), tsp A l1 l2 -> pmt A l1 l2
+| pmt2 : forall (l1 l2 l3 : list A), pmt A l1 l2 -> tsp A l2 l3 -> pmt A l1 l3.
+
+(** proof...  *)
+
+(** [] *)
+
+
+(** **** Exercise 8.5 *)
 
 Inductive par: Set := open | close.
 
@@ -105,18 +170,38 @@ Qed.
 
 
 
-(** * 8.3 Reasoning about Inductive Properties *)
 
+(** **** Exercise 8.12 *)
 
-(** **** Exercise 8.11 *)
-
-Theorem lt_le : forall n p : nat, n < p -> n <= p.
+Theorem le_my_le : forall n p : nat, n <= p -> my_le n p.
 Proof.
-  intros n p H. unfold lt in H.
-Admitted.
+  unfold my_le. intros n p np P Pn H.
+  elim np; trivial.
+  intros m nm Pm. apply H. assumption.
+Qed.  
 
 (** [] *)
 
+
+
+(** **** Exercise 8.13 *)
+
+Theorem le_trans' : forall n p q : nat, n <= p -> p <= q -> n <= q.
+Proof.
+  intros n p q np pq.
+  induction np as [|m nm IH]; trivial.
+  apply IH. apply le_Sn_le. assumption.
+Qed.
+
+Theorem my_le_trans : forall n p q : nat, my_le n p -> my_le p q -> my_le n q.
+Proof.
+  unfold my_le. intros n p q np pq.
+  intros P Pn H.
+  apply pq; try assumption.
+  apply np; try assumption.
+Qed.
+
+(** [] *)
 
 
 (** **** Exercise 8.14 *)
@@ -171,4 +256,169 @@ Proof.
     + apply le_n_S. assumption.
 Qed.
 
+(** [] *)
+
+
+(** **** Exercise 8.15 *)
+
+Inductive sorted (A : Set) (R : relation A) : list A -> Prop :=
+| sorted0 : sorted A R []
+| sorted1 : forall x : A, sorted A R [x]
+| sorted2 : forall (x y : A) (l : list A), 
+              R x y -> sorted A R (y::l) -> sorted A R (x::y::l).
+
+Definition sorted' (A : Set) (R : relation A) (l : list A) :=
+  forall (l1 l2 : list A) (n1 n2 : A),
+    l = l1 ++ (n1::n2::l2) -> R n1 n2.
+
+Theorem sorted_eq : forall (A : Set) (R : relation A) (l : list A),
+  sorted A R l <-> sorted' A R l.
+Proof.
+  intros A R l. split; intros H.
+  - (* -> *)
+    unfold sorted'.
+    induction H; intros l1 l2 n1 n2 H'.
+    + destruct l1; simpl in H'; discriminate H'.
+    + repeat (destruct l1; simpl in H'; try discriminate H').
+    + destruct l1 as [|h t].
+      * simpl in H'. injection H'.
+        intros H1 H2 H3. rewrite <- H2. rewrite <- H3. assumption.
+      * simpl in H'. injection H'.
+        intros H1 H2. apply (IHsorted t l2). assumption.
+  - (* <- *)
+    unfold sorted' in H.
+    induction l as [|h t]; try (constructor; fail).
+    destruct t as [|h' t']; try (constructor; fail).
+    apply sorted2.
+    + apply (H [] t'). reflexivity.
+    + apply IHt. intros l1 l2 n1 n2 H'.
+      apply (H (h::l1) l2). simpl.
+      rewrite H'. reflexivity.
+Qed.
+        
+
+(** [] *)
+
+
+(** **** Exercise 8.18 *)
+
+Section weird_induc_proof.
+
+Variable P : nat -> Prop.
+Variable f : nat -> nat.
+
+Hypothesis f_strict_mono : forall n p : nat, lt n p -> lt (f n) (f p).
+Hypothesis f_0 : lt 0 (f 0).
+
+Hypothesis P0 : P 0.
+Hypothesis P_Sn_n : forall n : nat, P (S n) -> P n.
+Hypothesis f_P : forall n : nat, P n -> P (f n).
+
+Lemma nltfn : forall n : nat, lt n (f n).
+Proof.
+  induction n as [|n'].
+  - assumption.
+  - unfold lt. unfold lt in IHn'.
+    apply le_trans with (m:= S (f n')).
+    + apply le_n_S. assumption.
+    + apply f_strict_mono. unfold lt. apply le_n.
+Qed.
+
+Lemma P_le : forall n m, n <= m -> P m -> P n.
+Proof.
+  intros n m nm Pm.
+  induction nm; trivial.
+  apply IHnm. apply P_Sn_n. assumption.
+Qed.
+
+Theorem weird_induc : forall n : nat, P n.
+Proof.
+  induction n as [|n'].
+  - assumption.
+  - apply (P_le _ (f n')).
+    + apply nltfn.
+    + apply f_P. assumption.
+Qed.
+
+End weird_induc_proof.
+
+(** [] *)
+
+
+(** **** Exercise 8.24 *)
+
+Inductive parse_rel : list par -> list par -> bin -> Prop :=
+  | parse_node : 
+      forall (l1 l2 l3 : list par) (t1 t2 : bin),
+        parse_rel l1 (close::l2) t1 -> parse_rel l2 l3 t2 ->
+        parse_rel (open::l1) l3 (N t1 t2)
+  | parse_leaf_nil :
+      parse_rel [] [] L
+  | parse_leaf_close :
+      forall l : list par, parse_rel (close::l) (close::l) L.
+
+Lemma parse_rel_sound_aux :
+  forall (l1 l2 : list par) (t : bin),
+    parse_rel l1 l2 t -> l1 = (bin_to_string t) ++ l2.
+Proof.
+  intros l1 l2 t H.
+  induction H.
+  - simpl. rewrite IHparse_rel1. rewrite IHparse_rel2.
+    rewrite <- app_assoc. simpl. reflexivity.
+  - trivial.
+  - trivial.
+Qed.
+
+Lemma parse_rel_sound :
+  forall l : list par, (exists t : bin, parse_rel l nil t) -> wp l.
+Proof.
+  intros l [t H].
+  rewrite (parse_rel_sound_aux l [] t H).
+  rewrite app_nil_r. apply wp_btos.
+Qed.
+
+(** [] *)
+
+
+Section little_semantics.
+
+Variables Var aExp bExp : Set.
+
+Inductive inst : Set :=
+| Skip : inst
+| Assign : Var -> aExp -> inst
+| Sequence : inst -> inst -> inst
+| WhileDo : bExp -> inst -> inst.
+
+Require Import ZArith.
+
+Variables 
+(state : Set)
+(update : state -> Var -> Z -> option state)
+(evalA : state -> aExp -> option Z)
+(evalB : state -> bExp -> option bool).
+
+
+
+(** **** Exercise 8.5 *)
+(** [] *)
+
+
+(** **** Exercise 8.5 *)
+(** [] *)
+
+
+(** **** Exercise 8.5 *)
+(** [] *)
+
+
+(** **** Exercise 8.5 *)
+(** [] *)
+
+
+(** **** Exercise 8.5 *)
+(** [] *)
+
+
+(** **** Exercise 8.5 *)
 (** [] *)
